funext and propext

theories/SetModel/HO_prop.v
@@ -22,36 +22,11 @@ Proof.
   + apply setMkPair_typing. apply four_typing. apply empty_in_univ.
 Qed.
 
-(* False proposition *)
+(* Proof irrelevance *)
 
-Definition falseTy_HO : ZFSet -> ZFSet := fun γ => prop FalseS.
-
-Lemma falseTy_HO_typing (Γ : ZFSet) : ∀ γ ∈ Γ, falseTy_HO γ ∈ Ω.
+Definition propTy_HO_irr {Γ : ZFSet} {P p q : ZFSet -> ZFSet} (HP : ∀ γ ∈ Γ, P γ ∈ Ω) (Hp : ∀ γ ∈ Γ, p γ ∈ P γ)
+  (Hq : ∀ γ ∈ Γ, q γ ∈ P γ) : ∀ γ ∈ Γ, p γ ≡ q γ.
 Proof.
-  intros. cbn. apply prop_typing.
-Qed.
-
-(* Eliminator of False *)
-
-Definition emptyrecTm_HO (A : ZFSet -> ZFSet) (H : ZFSet -> ZFSet) := ∅.
-
-Lemma emptyrecTm_HO_typing {n : nat} {Γ : ZFSet} {A H : ZFSet -> ZFSet}
-  (HA : ∀ γ ∈ Γ, A γ ∈ 𝕌 n) (HH : ∀ γ ∈ Γ, H γ ∈ falseTy_HO γ) :
-  ∀ γ ∈ Γ, emptyrecTm_HO A H ∈ 𝕌el n (A γ).
-Proof.
-  intros γ Hγ. specialize (HH γ Hγ). cbn in HH. apply prop_true_if in HH. destruct HH.
-Qed.
-
-(* Observational equality *)
-
-Definition eqTy_HO (A t u : ZFSet -> ZFSet) : ZFSet -> ZFSet :=
-  fun γ => prop (t γ ≡ u γ).
-
-Definition reflTm_HO (A t : ZFSet -> ZFSet) : ZFSet -> ZFSet := fun _ => ∅.
-
-Lemma eqTy_HO_typing {n : nat} {Γ : ZFSet} {A t u : ZFSet -> ZFSet}
-  (HA : ∀ γ ∈ Γ, A γ ∈ 𝕌 n) (Ht : ∀ γ ∈ Γ, t γ ∈ 𝕌el n (A γ)) (Hu : ∀ γ ∈ Γ, u γ ∈ 𝕌el n (A γ)) :
-  ∀ γ ∈ Γ, eqTy_HO A t u γ ∈ Ω.
-Proof.
-  intros γ Hγ. cbn. apply prop_typing.
+  intros γ Hγ. specialize (HP γ Hγ). specialize (Hp γ Hγ). specialize (Hq γ Hγ). cbn in *.
+  refine (trans _ (sym _)). now apply (proof_irr HP). now apply (proof_irr HP).
 Qed.
