theories/SetModel/HO_forall.v
@@ -1,0 +1,75 @@
+Require Import library.
+Require Import ZF_axioms ZF_library ZF_nat.
+Require Import HO HO_prop HO_univ HO_box.
+
+(* Proof-irrelevant pi types *)
+
+Definition forallTy_HO (n : nat) (A : ZFSet -> ZFSet) (B : ZFSet -> ZFSet) : ZFSet -> ZFSet :=
+  fun γ => prop (∀ a ∈ 𝕌el n (A γ), ∅ ∈ B ⟨ γ ; a ⟩).
+
+Lemma forallTy_HO_typing {n : nat} {Γ : ZFSet} {A : ZFSet -> ZFSet} {B : ZFSet -> ZFSet}
+  (HA : ∀ γ ∈ Γ, A γ ∈ 𝕌 n) (HB : ∀ γa ∈ ctxExt n Γ A, B γa ∈ Ω) :
+  ∀ γ ∈ Γ, forallTy_HO n A B γ ∈ Ω.
+Proof.
+  intros γ Hγ. unfold forallTy_HO. apply prop_typing.
+Qed.
+
+(* Lambda abstraction *)
+
+Definition ilamTm_HO (n : nat) (A t : ZFSet -> ZFSet) : ZFSet -> ZFSet := fun γ => ∅.
+
+Lemma lamTm_HO_typing (n : nat) {Γ : ZFSet} {A B t : ZFSet -> ZFSet}
+  (HA : ∀ γ ∈ Γ, A γ ∈ 𝕌 n) (HB : ∀ γa ∈ ctxExt n Γ A, B γa ∈ Ω)
+  (Ht : ∀ γa ∈ ctxExt n Γ A, t γa ∈ B γa) :
+  ∀ γ ∈ Γ, ilamTm_HO n A t γ ∈ forallTy_HO n A B γ.
+Proof.
+  intros γ Hγ. cbn. unfold ilamTm_HO. unfold forallTy_HO.
+  apply prop_true_iff. intros a Ha. assert (⟨ γ ; a ⟩ ∈ ctxExt n Γ A) as Hγa.
+  { apply setMkSigma_typing ; try assumption. intros γ' Hγ'. apply 𝕌el_typing. now apply HA. }
+  specialize (Ht _ Hγa). cbn in Ht. specialize (HB _ Hγa). cbn in HB.
+  refine (proof_irr' HB _ Ht).
+Qed.
+
+(* Application *)
+
+Definition iappTm_HO (n : nat) (A t u : ZFSet -> ZFSet) : ZFSet -> ZFSet := fun γ => ∅.
+
+Lemma appTm_HO_typing (n : nat) {Γ : ZFSet} {A B t u : ZFSet -> ZFSet} 
+  (HA : ∀ γ ∈ Γ, A γ ∈ 𝕌 n) (HB : ∀ γa ∈ ctxExt n Γ A, B γa ∈ Ω)
+  (Ht : ∀ γ ∈ Γ, t γ ∈ forallTy_HO n A B γ) (Hu : ∀ γ ∈ Γ, u γ ∈ 𝕌el n (A γ)) :
+  ∀ γ ∈ Γ, iappTm_HO n A t u γ ∈ B ⟨ γ ; u γ ⟩.
+Proof.
+  intros γ Hγ. cbn. unfold iappTm_HO. 
+  specialize (Ht _ Hγ). cbn in Ht. unfold forallTy_HO in Ht. apply prop_true_if in Ht.
+  apply Ht. now apply Hu.
+Qed.
+
+(* Implication *)
+
+Definition implTy_HO' (Γ : ZFSet) (P : ZFSet -> ZFSet) (Q : ZFSet -> ZFSet) : ZFSet -> ZFSet :=
+  forallTy_HO 0 (boxTy_HO P) (fun γa => Q (ctx_wk 0 Γ (boxTy_HO P) γa)).
+
+Definition implTy_HO (P : ZFSet -> ZFSet) (Q : ZFSet -> ZFSet) : ZFSet -> ZFSet :=
+  fun γ => prop (P γ ⊂ Q γ).
+
+Lemma implTy_HO_typing {Γ : ZFSet} {P : ZFSet -> ZFSet} {Q : ZFSet -> ZFSet}
+  (HP : ∀ γ ∈ Γ, P γ ∈ Ω) (HQ : ∀ γ ∈ Γ, Q γ ∈ Ω) : ∀ γ ∈ Γ, implTy_HO P Q γ ∈ Ω.
+Proof.
+  intros. now apply prop_typing.
+Qed.
+
+Lemma implTy_HO_eq_implTy_HO' {Γ : ZFSet} {P : ZFSet -> ZFSet} {Q : ZFSet -> ZFSet}
+  (HP : ∀ γ ∈ Γ, P γ ∈ Ω) (HQ : ∀ γ ∈ Γ, Q γ ∈ Ω) : ∀ γ ∈ Γ, implTy_HO P Q γ ≡ implTy_HO' Γ P Q γ.
+Proof.
+  intros γ Hγ. unfold implTy_HO. unfold implTy_HO'. unfold forallTy_HO.
+  apply (fstS prop_ext). split.
+  - intros H x Hx. refine (transpS (fun X => ∅ ∈ Q X) (sym _) _).
+    { apply ctxExtβ1 ; try assumption. intros γ' Hγ'. now apply (boxTy_HO_typing (Γ := Γ)). }
+    apply H. eapply proof_irr'. now apply HP. exact (transpS (fun X => _ ∈ X) (el_boxTy HP γ Hγ) Hx).
+  - intros H x Hx. pose proof (sym (proof_irr (HP γ Hγ) x Hx)) as H0. destruct H0.
+    specialize (H ∅ (transpS (fun X => _ ∈ X) (sym (el_boxTy HP γ Hγ)) Hx)).
+    refine (transpS (fun X => ∅ ∈ Q X) _ H).
+    apply ctxExtβ1 ; try assumption. intros γ' Hγ'. now apply (boxTy_HO_typing (Γ := Γ)).
+    refine (transpS (fun X => _ ∈ X) (sym (el_boxTy HP γ Hγ)) Hx).
+Qed.
+    
